Work on irrelevant store questions (c) and (d), and refactoring

disjoint.v
@@ -1,11 +1,7 @@
 Require Import FunInd.
 Require Import FunctionalExtensionality.
-Require Import Ensembles.
-
-Arguments Empty_set {U}.
-Arguments Singleton {U}.
-Arguments Union {U}.
-Arguments Included {U}.
+Require Import Nat.
+Require Import Specif.
 
 Inductive expr : Set :=
   | e_n : nat -> expr
@@ -14,14 +10,18 @@ Inductive expr : Set :=
   | e_assgn : nat -> expr -> expr
   | e_seq : expr -> expr -> expr.
 
-Fixpoint loc (e : expr) : Ensemble nat :=
+Fixpoint loc (e : expr) : nat -> bool :=
+  fun l' =>
   match e with
-  | e_n _ => Empty_set
-  | e_skip => Empty_set
-  | e_deref l => Singleton l
-  | e_assgn l e => Union (Singleton l) (loc e)
-  | e_seq e1 e2 => Union (loc e1) (loc e2)
+  | e_n _ => false
+  | e_skip => false
+  | e_deref l => l =? l'
+  | e_assgn l e => if l =? l' then true else loc e l'
+  | e_seq e1 e2 => if loc e1 l' then true else loc e2 l'
   end.
+
+Definition subset (s0 s1 : nat -> bool) : Prop :=
+  forall l, s0 l = true -> s1 l = true.
 
 Module S.
   Definition t := nat -> option nat.
@@ -31,10 +31,10 @@ Module S.
   Definition get (s : t) l := s l.
 
   Definition remove (s : t) (l : nat) : t :=
-    fun l' => if Nat.eqb l l' then None else get s l'.
+    fun l' => if l =? l' then None else get s l'.
 
   Definition add (s : t) (l : nat) (n : nat) : t :=
-    fun l' => if Nat.eqb l l' then Some n else get s l'.
+    fun l' => if l =? l' then Some n else get s l'.
 
   Definition dom (s : t) : nat -> bool :=
     fun l => match get s l with
@@ -42,16 +42,20 @@ Module S.
       | Some _ => true
       end.
 
-  Lemma get_eq_domain : forall s l v, get s l = Some v -> dom s l = true.
+  Lemma get_eq_dom : forall s l v,
+    get s l = v ->
+    dom s l = (match v with None => false | Some _ => true end).
   Proof.
-    intros. unfold dom. rewrite H. reflexivity.
+    intros. unfold dom. subst. reflexivity.
   Qed.
 
-  Lemma domain_eq_get : forall s l, dom s l = true -> exists v, get s l = Some v.
+  Lemma dom_eq_get : forall s l b,
+    dom s l = b ->
+    (match b with false => get s l = None | true => exists v, get s l = Some v end).
   Proof.
-    intros. unfold dom in H. unfold get in H. case (s l) eqn:H1 in H.
+    intros. unfold dom in H. unfold get in H. case (s l) eqn:H1 in H; subst.
     - exists n. unfold get. assumption.
-    - inversion H.
+    - assumption.
   Qed.
 
   Lemma disjoint_absurd : forall s0 s1 l v0 v1,
@@ -60,8 +64,8 @@ Module S.
     dom s0 l = false \/ dom s1 l = false -> False.
   Proof.
     intros. destruct H1.
-    - apply get_eq_domain in H. rewrite H in H1. inversion H1.
-    - apply get_eq_domain in H0. rewrite H0 in H1. inversion H1.
+    - apply get_eq_dom in H. rewrite H in H1. inversion H1.
+    - apply get_eq_dom in H0. rewrite H0 in H1. inversion H1.
   Qed.
 
   Definition disjoint_union (s0 s1 : t) : nat -> option nat :=
@@ -76,28 +80,28 @@ End S.
 
 Notation "f + g" := (S.disjoint_union f g).
 
-Inductive transition e0 s0 e1 s1 : Prop :=
-  | t_deref : forall l n,
+Inductive transition : expr -> S.t -> expr -> S.t -> Prop :=
+  | t_deref : forall e0 s0 e1 s1 l n,
       e0 = e_deref l ->
       e1 = e_n n ->
       Some n = S.get s0 l ->
       s0 = s1 ->
       transition e0 s0 e1 s1
-  | t_assgn1 : forall l n,
+  | t_assgn1 : forall e0 s0 e1 s1 l n,
       e0 = e_assgn l (e_n n) ->
       e1 = e_skip ->
       s1 = S.add s0 l n ->
       transition e0 s0 e1 s1
-  | t_assgn2 : forall l e0' e1',
+  | t_assgn2 : forall e0 s0 e1 s1 l e0' e1',
       e0 = e_assgn l e0' ->
       e1 = e_assgn l e1' ->
       transition e0' s0 e1' s1 ->
       transition e0 s0 e1 s1
-  | t_seq1 :
+  | t_seq1 : forall e0 s0 e1 s1,
       e0 = e_seq e_skip e1 ->
       s0 = s1 ->
       transition e0 s0 e1 s1
-  | t_seq2 : forall e0' e1' e'',
+  | t_seq2 : forall e0 s0 e1 s1 e0' e1' e'',
       e0 = e_seq e0' e'' ->
       e1 = e_seq e1' e'' ->
       transition e0' s0 e1' s1 ->
@@ -110,31 +114,78 @@ Lemma one_step_determinacy_expr : forall e s e0 s0 e1 s1,
   [e, s] ~> [e0, s0] -> [e, s] ~> [e1, s1] -> [e0, s0] = [e1, s1].
 Proof.
   intros e s.
-  induction e;
-  intros e' s' e'' s'' Hl Hr;
-  inversion Hl; inversion Hr; try discriminate.
-  - split.
-    + rewrite H0. rewrite H4. f_equal. rewrite H in H3. inversion H3.
-    rewrite <- H8 in H5. rewrite <- H1 in H5. inversion H5. reflexivity.
-    + rewrite H2 in H6. exact H6.
-  - split.
-    + rewrite H0. rewrite H3. reflexivity.
-    + inversion H. inversion H2. rewrite H6 in H8. rewrite H7 in H9. inversion H9.
-      rewrite <- H8 in H4. rewrite H10 in H1. rewrite <- H1 in H4. symmetry. exact H4.
-  - inversion H. inversion H2. rewrite H7 in H9. rewrite <- H9 in H4. inversion H4; discriminate.
-  - inversion H. inversion H2. rewrite H9 in H7. rewrite <- H7 in H1. inversion H1; discriminate.
-  - inversion H. inversion H2. rewrite <- H7 in H1. rewrite <- H9 in H4.
+  induction e; intros e' s' e'' s'' Hl Hr;
+  inversion Hl; inversion Hr; try discriminate; subst.
+  - rewrite H in H7. inversion H7. rewrite H2 in H1.
+    rewrite <- H1 in H9. inversion H9. constructor; reflexivity.
+  - rewrite H in H6. inversion H6. constructor; reflexivity.
+  - inversion H; inversion H6; subst. inversion H8; discriminate.
+  - inversion H; inversion H6; subst. inversion H1; discriminate.
+  - inversion H; inversion H6; subst.
     apply (IHe e1' s' e1'0 s'') in H1.
-    + inversion H1. rewrite H5 in H0. rewrite H6 in H8. rewrite H8 in H0. rewrite H0. rewrite H3.
-      rewrite H10. auto.
+    + inversion H1; subst. constructor; reflexivity.
     + assumption.
-  - inversion H. inversion H1. rewrite <- H5. rewrite H7.
-    rewrite H2 in H0. rewrite H0. auto.
-  - inversion H. inversion H1. rewrite H5 in H7. rewrite <- H7 in H3. inversion H3; discriminate.
-  - inversion H. inversion H2. rewrite H7 in H5. rewrite <- H5 in H1. inversion H1; discriminate.
-  - inversion H. inversion H2. rewrite <- H6 in H1. rewrite <- H8 in H4.
+  - inversion H; subst. inversion H5. constructor; reflexivity.
+  - inversion H; subst. inversion H5; subst. inversion H7; discriminate.
+  - inversion H; inversion H6; subst. inversion H1; discriminate.
+  - inversion H; subst. inversion H6; subst.
     apply (IHe1 e1' s' e1'0 s'') in H1.
-    + inversion H1. rewrite H5 in H0. rewrite H7 in H9. rewrite H9 in H0. rewrite H0. rewrite H3.
-      rewrite H10. auto.
+    + inversion H1; subst. constructor; reflexivity.
     + assumption.
 Qed.
+
+Lemma store_get_disjoint : forall s s' l n,
+  Some n = S.get s l -> S.dom s' l = false -> Some n = S.get (s + s') l.
+Proof.
+  intros.
+  apply (S.dom_eq_get s' l false) in H0.
+  unfold S.get. unfold S.disjoint_union.
+  rewrite <- H. rewrite H0. reflexivity.
+Qed.
+
+(* Requires function extensionality to show equality of stores *)
+Lemma store_add_disjoint : forall s s' l n,
+  S.dom s' l = false -> S.add s l n + s' = S.add (s + s') l n.
+Proof.
+  intros.
+  apply (S.dom_eq_get s' l false) in H.
+  unfold S.add. unfold S.disjoint_union.
+Admitted.
+
+Lemma irrelevant_store_can_be_added : forall e s e1 s1 s0,
+  [e, s] ~> [e1, s1] ->
+  (forall l, S.dom s0 l = false \/ S.dom s1 l = false) ->
+  [e, s + s0] ~> [e1, s1 + s0].
+Proof.
+  intros.
+  induction H; subst.
+  - apply (t_deref _ _ _ _ l n); try reflexivity.
+    specialize (H0 l). destruct H0 as [Hs0|Hs1].
+    + apply (store_get_disjoint s2 s0 l n); assumption.
+    + apply (S.dom_eq_get s2 l false) in Hs1.
+      rewrite <- H2 in Hs1. discriminate.
+  - apply (t_assgn1 _ _ _ _ l n); try reflexivity.
+    specialize (H0 l). destruct H0 as [Hs0|Hs1].
+    +
+Admitted.
+
+Lemma nat_eqb_refl : forall x, (x =? x) = true.
+Proof.
+  intros. induction x.
+  - unfold Nat.eqb. reflexivity.
+  - unfold Nat.eqb. apply IHx.
+Qed.
+
+Lemma irrelevant_store_can_be_removed : forall e s s0 e1 s1,
+  [e, s + s0] ~> [e1, s1] ->
+  (subset (loc e) (S.dom s)) ->
+  exists s', [e, s] ~> [e1, s'] /\ s1 = s' + s0.
+Proof.
+  intros. induction H.
+  - exists s. split.
+    + rewrite H. rewrite H1. apply (t_deref (e_deref l) s (e_n n) s l n); try reflexivity.
+      cut (S.dom s l = true).
+      *intros.
+        apply S.dom_eq_get in H4. destruct H4.
+        rewrite H4.
+Admitted.
